Fee devision in SendToChain added. Module UInt256.fst has been changed using UIntN.fstp and UIntN.fstip files from official repo.

FStar.UInt256.fst
@@ -1,140 +1,250 @@
+/// For FStar.UIntN.fstp: anything that you fix/update here should be
+/// reflected in [FStar.IntN.fstp], which is mostly a copy-paste of
+/// this module.
+///
+/// Except, as compared to [FStar.IntN.fstp], here:
+///  - every occurrence of [int_t] has been replaced with [uint_t]
+///  - every occurrence of [@%] has been replaced with [%].
+///  - some functions (e.g., add_underspec, etc.) are only defined here, not on signed integers
+
+/// This module provides an abstract type for machine integers of a
+/// given signedness and width. The interface is designed to be safe
+/// with respect to arithmetic underflow and overflow.
+
+/// Note, we have attempted several times to re-design this module to
+/// make it more amenable to normalization and to impose less overhead
+/// on the SMT solver when reasoning about machine integer
+/// arithmetic. The following github issue reports on the current
+/// status of that work.
+///
+/// https://github.com/FStarLang/FStar/issues/1757
 module FStar.UInt256
-
-let n = 256
-
 open FStar.UInt
 open FStar.Mul
 
-(* NOTE: anything that you fix/update here should be reflected in [FStar.IntN.fstp], which is mostly
- * a copy-paste of this module. *)
+let n = 256
 
-(* This is really the same thing as [FStar.IntN.fstp], with:
- * - every occurrence of [int_t] has been replaced with [uint_t]
- * - every occurrence of [@%] has been replaced with [%].
- *)
+type t : eqtype =
+  | Mk: v:uint_t n -> t
 
-private type t' = | Mk: v:uint_t n -> t'
-type t = t'
+#set-options "--max_fuel 0 --max_ifuel 0"
 
-let v (x:t) : Tot (uint_t n) = x.v
+(** A coercion that projects a bounded mathematical integer from a
+    machine integer *)
+val v (x:t) : Tot (uint_t n)
+let v x = x.v
 
-val add: a:t -> b:t -> Pure t
+(** A coercion that injects a bounded mathematical integers into a
+    machine integer *)
+val uint_to_t (x:uint_t n) : Pure t
+  (requires True)
+  (ensures (fun y -> v y = x))
+
+irreducible
+let uint_to_t x = Mk x
+
+
+(** Injection/projection inverse *)
+val uv_inv (x : t) : Lemma
+  (ensures (uint_to_t (v x) == x))
+  [SMTPat (v x)]
+
+let uv_inv _ = ()
+
+(** Projection/injection inverse *)
+val vu_inv (x : uint_t n) : Lemma
+  (ensures (v (uint_to_t x) == x))
+  [SMTPat (uint_to_t x)]
+let vu_inv _ = ()
+
+(** An alternate form of the injectivity of the [v] projection *)
+val v_inj (x1 x2: t): Lemma
+  (requires (v x1 == v x2))
+  (ensures (x1 == x2))
+let v_inj _ _ = ()
+
+(** Constants 0 and 1 *)
+val zero : x:t{v x = 0}
+let zero = uint_to_t 0
+
+
+(**** Addition primitives *)
+
+(** Bounds-respecting addition
+
+    The precondition enforces that the sum does not overflow,
+    expressing the bound as an addition on mathematical integers *)
+val add (a:t) (b:t) : Pure t
   (requires (size (v a + v b) n))
   (ensures (fun c -> v a + v b = v c))
-let add a b =
-  Mk (add (v a) (v b))
+let add a b = Mk (add (v a) (v b))
 
-val add_underspec: a:t -> b:t -> Pure t
+(** Underspecified, possibly overflowing addition:
+
+    The postcondition only enures that the result is the sum of the
+    arguments in case there is no overflow *)
+val add_underspec (a:t) (b:t) : Pure t
   (requires True)
   (ensures (fun c ->
     size (v a + v b) n ==> v a + v b = v c))
-let add_underspec a b =
-  Mk (add_underspec (v a) (v b))
+let add_underspec a b = Mk (add_underspec (v a) (v b))
 
-val add_mod: a:t -> b:t -> Pure t
+(** Addition modulo [2^n]
+
+    Machine integers can always be added, but the postcondition is now
+    in terms of addition modulo [2^n] on mathematical integers *)
+val add_mod (a:t) (b:t) : Pure t
   (requires True)
-  (ensures (fun c -> (v a + v b) % pow2 n = v c))
-let add_mod a b =
-  Mk (add_mod (v a) (v b))
+  (ensures (fun c -> FStar.UInt.add_mod (v a) (v b) = v c))
+let add_mod a b = Mk (add_mod (v a) (v b))
 
-(* Subtraction primitives *)
-val sub: a:t -> b:t -> Pure t
+(**** Subtraction primitives *)
+
+
+(** Bounds-respecting subtraction
+
+    The precondition enforces that the difference does not underflow,
+    expressing the bound as a difference on mathematical integers *)
+val sub (a:t) (b:t) : Pure t
   (requires (size (v a - v b) n))
   (ensures (fun c -> v a - v b = v c))
-let sub a b =
-  Mk (sub (v a) (v b))
+let sub a b = Mk (sub (v a) (v b))
 
-val sub_underspec: a:t -> b:t -> Pure t
+(** Underspecified, possibly overflowing subtraction:
+
+    The postcondition only enures that the result is the difference of
+    the arguments in case there is no underflow *)
+val sub_underspec (a:t) (b:t) : Pure t
   (requires True)
   (ensures (fun c ->
     size (v a - v b) n ==> v a - v b = v c))
-let sub_underspec a b =
-  Mk (sub_underspec (v a) (v b))
+let sub_underspec a b = Mk (sub_underspec (v a) (v b))
 
-val sub_mod: a:t -> b:t -> Pure t
+(** Subtraction modulo [2^n]
+
+    Machine integers can always be subtractd, but the postcondition is
+    now in terms of subtraction modulo [2^n] on mathematical integers *)
+val sub_mod (a:t) (b:t) : Pure t
   (requires True)
-  (ensures (fun c -> (v a - v b) % pow2 n = v c))
-let sub_mod a b =
-  Mk (sub_mod (v a) (v b))
+  (ensures (fun c -> FStar.UInt.sub_mod (v a) (v b) = v c))
+let sub_mod a b = Mk (sub_mod (v a) (v b))
 
-(* Multiplication primitives *)
-val mul: a:t -> b:t -> Pure t
+(**** Multiplication primitives *)
+
+
+(** Bounds-respecting multiplication
+
+    The precondition enforces that the product does not overflow,
+    expressing the bound as a product on mathematical integers *)
+val mul (a:t) (b:t) : Pure t
   (requires (size (v a * v b) n))
   (ensures (fun c -> v a * v b = v c))
-let mul a b =
-  Mk (mul (v a) (v b))
+let mul a b = Mk (mul (v a) (v b))
 
-val mul_underspec: a:t -> b:t -> Pure t
+(** Underspecified, possibly overflowing product
+
+    The postcondition only enures that the result is the product of
+    the arguments in case there is no overflow *)
+val mul_underspec (a:t) (b:t) : Pure t
   (requires True)
   (ensures (fun c ->
     size (v a * v b) n ==> v a * v b = v c))
-let mul_underspec a b =
-  Mk (mul_underspec (v a) (v b))
+let mul_underspec a b = Mk (mul_underspec (v a) (v b))
 
-val mul_mod: a:t -> b:t -> Pure t
+(** Multiplication modulo [2^n]
+
+    Machine integers can always be multiplied, but the postcondition
+    is now in terms of product modulo [2^n] on mathematical integers *)
+val mul_mod (a:t) (b:t) : Pure t
   (requires True)
-  (ensures (fun c -> (v a * v b) % pow2 n = v c))
-let mul_mod a b =
-  Mk (mul_mod (v a) (v b))
+  (ensures (fun c -> FStar.UInt.mul_mod (v a) (v b) = v c))
+let mul_mod a b = Mk (mul_mod (v a) (v b))
 
-(* Division primitives *)
-val div: a:t -> b:t{v b <> 0} -> Pure t
-  (requires (size (v a / v b) n))
-  (ensures (fun c -> v b <> 0 ==> v a / v b = v c))
-let div a b =
-  Mk (div (v a) (v b))
+(**** Division primitives *)
+//--split_queries always
+(** Euclidean division of [a] and [b], with [b] non-zero *)
+val div (a:t) (b:t{v b <> 0}) : Pure t
+  (requires (True))
+  (ensures (fun c -> v a / v b = v c))
+let div a b = Mk (div (v a) (v b))
 
-val div_underspec: a:t -> b:t{v b <> 0} -> Pure t
+(**** Modulo primitives *)
+
+(** Euclidean remainder
+
+    The result is the modulus of [a] with respect to a non-zero [b] *)
+val rem (a:t) (b:t{v b <> 0}) : Pure t
   (requires True)
-  (ensures (fun c ->
-    (v b <> 0 /\ size (v a / v b) n) ==> v a / v b = v c))
-let div_underspec a b =
-  Mk (div_underspec (v a) (v b))
-
-(* Modulo primitives *)
-val rem: a:t -> b:t{v b <> 0} -> Pure t
-  (requires True)
-  (ensures (fun c ->
-    v a - ((v a / v b) * v b) = v c))
+  (ensures (fun c -> FStar.UInt.mod (v a) (v b) = v c))
 let rem a b = Mk (mod (v a) (v b))
 
-(* Bitwise operators *)
-val logand: t -> t -> Tot t
-let logand a b = Mk (logand (v a) (v b))
-val logxor: t -> t -> Tot t
-let logxor a b = Mk (logxor (v a) (v b))
-val logor: t -> t -> Tot t
-let logor a b = Mk (logor (v a) (v b))
-val lognot: t -> Tot t
-let lognot a = Mk (lognot (v a))
+(**** Bitwise operators *)
 
-val uint_to_t: x:(uint_t n) -> Pure t
-  (requires True)
-  (ensures (fun y -> v y = x))
-let uint_to_t x = Mk x
+/// Also see FStar.BV
 
-(* Shift operators *)
-val shift_right: a:t -> s:UInt32.t -> Pure t
+(** Bitwise logical conjunction *)
+val logand (x:t) (y:t) : Pure t
   (requires True)
-  (ensures (fun c -> UInt32.v s < n ==> v c = (v a / (pow2 (UInt32.v s)))))
+  (ensures (fun z -> v x `logand` v y = v z))
+let logand x y = Mk (logand (v x) (v y))
+
+(** Bitwise logical exclusive-or *)
+val logxor (x:t) (y:t) : Pure t
+  (requires True)
+  (ensures (fun z -> v x `logxor` v y == v z))
+let logxor x y = Mk (logxor (v x) (v y))
+
+(** Bitwise logical disjunction *)
+val logor (x:t) (y:t) : Pure t
+  (requires True)
+  (ensures (fun z -> v x `logor` v y == v z))
+let logor x y = Mk (logor (v x) (v y))
+
+(** Bitwise logical negation *)
+val lognot (x:t) : Pure t
+  (requires True)
+  (ensures (fun z -> lognot (v x) == v z))
+let lognot x = Mk (lognot (v x))
+
+(**** Shift operators *)
+
+(** Shift right with zero fill, shifting at most the integer width *)
+val shift_right (a:t) (s:UInt32.t) : Pure t
+  (requires (UInt32.v s < n))
+  (ensures (fun c -> FStar.UInt.shift_right (v a) (UInt32.v s) = v c))
 let shift_right a s = Mk (shift_right (v a) (UInt32.v s))
 
-val shift_left: a:t -> s:UInt32.t -> Pure t
-  (requires True)
-  (ensures (fun c -> UInt32.v s < n ==> v c = ((v a * pow2 (UInt32.v s)) % pow2 n)))
+#push-options "--z3rlimit 80 --fuel 1"  //AR: working around the interleaving semantics of pragmas
+(** Shift left with zero fill, shifting at most the integer width *)
+val shift_left (a:t) (s:UInt32.t) : Pure t
+  (requires (UInt32.v s < n))
+  (ensures (fun c -> FStar.UInt.shift_left (v a) (UInt32.v s) = v c))
 let shift_left a s = Mk (shift_left (v a) (UInt32.v s))
 
-(* Comparison operators *)
+(**** Comparison operators *)
+
+(** Equality
+
+    Note, it is safe to also use the polymorphic decidable equality
+    operator [=] *)
 let eq (a:t) (b:t) : Tot bool = eq #n (v a) (v b)
+
+(** Greater than *)
 let gt (a:t) (b:t) : Tot bool = gt #n (v a) (v b)
+
+(** Greater than or equal *)
 let gte (a:t) (b:t) : Tot bool = gte #n (v a) (v b)
+
+(** Less than *)
 let lt (a:t) (b:t) : Tot bool = lt #n (v a) (v b)
+
+(** Less than or equal *)
 let lte (a:t) (b:t) : Tot bool = lte #n (v a) (v b)
 
-assume val eq_mask: a:t -> b:t -> Tot (c:t{(v a = v b ==> v c = pow2 n - 1) /\ (v a <> v b ==> v c = 0)})
-assume val gte_mask: a:t -> b:t -> Tot (c:t{(v a >= v b ==> v c = pow2 n - 1) /\ (v a < v b ==> v c = 0)})
 
-(* Infix notations *)
+#pop-options
+
+(*** Infix notations *)
 unfold let op_Plus_Hat = add
 unfold let op_Plus_Question_Hat = add_underspec
 unfold let op_Plus_Percent_Hat = add_mod
@@ -157,6 +267,32 @@ unfold let op_Greater_Equals_Hat = gte
 unfold let op_Less_Hat = lt
 unfold let op_Less_Equals_Hat = lte
 
-(* To input / output constants *)
-assume val to_string: t -> Tot string
-assume val of_string: string -> Tot t
+(**** To input / output constants *)
+(** In decimal representation *)
+val to_string: t -> Tot string
+let to_string _ = admit ()
+
+(** In hex representation (with leading 0x) *)
+val to_string_hex: t -> Tot string
+let to_string_hex _ = admit ()
+
+(** In fixed-width hex representation (left-padded with zeroes, no leading 0x) *)
+val to_string_hex_pad: t -> Tot string
+let to_string_hex_pad _ = admit ()
+
+val of_string: string -> Tot t
+let of_string _ = admit ()
+
+#set-options "--lax"
+//This private primitive is used internally by the
+//compiler to translate bounded integer constants
+//with a desugaring-time check of the size of the number,
+//rather than an expensive verification check.
+//Since it is marked private, client programs cannot call it directly
+//Since it is marked unfold, it eagerly reduces,
+//eliminating the verification overhead of the wrapper
+private
+unfold
+let __uint_to_t (x:int) : Tot t
+    = uint_to_t x
+#reset-options
